@prefix dct: <http://purl.org/dc/terms/> .
@prefix prov: <http://www.w3.org/ns/prov#> .
@prefix rdfs: <http://www.w3.org/2000/01/rdf-schema#> .
@prefix skos: <http://www.w3.org/2004/02/skos/core#> .
@prefix tair: <http://openscience.adaptcentre.ie/ontologies/tair/> .

tair:AccessToEducationAndTrainingAiSystem a tair:Concept ;
    dct:source <https://eur-lex.europa.eu/legal-content/EN/TXT/HTML/?uri=CELEX:52021PC0206&from=EN> ;
    skos:broader tair:EducationAndTrainingHighRiskAreas ;
    skos:definition "AI systems intended to be used for the purpose of determining access or assigning natural persons to educational and vocational training institutions;"@en ;
    skos:prefLabel "access to education and vocational training"@en .

tair:AdministrationOfJusticeAndDemocraticHighRiskArea a tair:Concept ;
    dct:source <https://eur-lex.europa.eu/legal-content/EN/TXT/HTML/?uri=CELEX:52021PC0206&from=EN> ;
    skos:definition "Administration of justice and democratic processes:"@en ;
    skos:prefLabel "administration of justice and democratic processes"@en ;
    skos:related tair:AiSystem .

tair:AgriculturalAndForsetryVehiclesHarmonisedLegislation a tair:Concept ;
    dct:source <https://eur-lex.europa.eu/legal-content/EN/TXT/HTML/?uri=CELEX:52021PC0206&from=EN> ;
    skos:definition "Regulation (EU) No 167/2013 of the European Parliament and of the Council of 5 February 2013 on the approval and market surveillance of agricultural and forestry vehicles (OJ L 60, 2.3.2013, p. 1);"@en ;
    skos:prefLabel "agricultural and forestry vehicles harmonised legislation"@en .

tair:AssessmentInEducationAndTrainingAiSystem a tair:Concept ;
    dct:source <https://eur-lex.europa.eu/legal-content/EN/TXT/HTML/?uri=CELEX:52021PC0206&from=EN> ;
    skos:broader tair:EducationAndTrainingHighRiskAreas ;
    skos:definition "AI systems intended to be used for the purpose of assessing students in educational and vocational training institutions and for assessing participants in tests commonly required for admission to educational institutions."@en ;
    skos:prefLabel "assessment in education and vocational training"@en .

tair:AuthorisedRepresentative a tair:Concept ;
    dct:source <https://eur-lex.europa.eu/legal-content/EN/TXT/HTML/?uri=CELEX:52021PC0206&from=EN> ;
    skos:broader tair:Operator ;
    skos:definition "any natural or legal person established in the Union who has received a written mandate from a provider of an AI system to, respectively, perform and carry out on its behalf the obligations and procedures established by this Regulation"@en ;
    skos:prefLabel "authorised representative"@en ;
    skos:related tair:Provider .

tair:BiometricCategorisationSystem a tair:Concept ;
    dct:source <https://eur-lex.europa.eu/legal-content/EN/TXT/HTML/?uri=CELEX:52021PC0206&from=EN> ;
    skos:broader tair:AiSystem ;
    skos:definition "an AI system for the purpose of assigning natural persons to specific categories, such as sex, age, hair colour, eye colour, tattoos, ethnic origin or sexual or political orientation, on the basis of their biometric data"@en ;
    skos:prefLabel "biometric categorisation system"@en ;
    skos:related tair:BiometricData .

tair:BiometricIdHighRiskArea a tair:Concept ;
    dct:source <https://eur-lex.europa.eu/legal-content/EN/TXT/HTML/?uri=CELEX:52021PC0206&from=EN> ;
    skos:definition "Biometric identification and categorisation of natural persons"@en ;
    skos:prefLabel "biometric identification and categorisation of natural persons"@en ;
    skos:related tair:AiSystem .

tair:BurningGaseousFuelsHarmonisedLegislation a tair:Concept ;
    dct:source <https://eur-lex.europa.eu/legal-content/EN/TXT/HTML/?uri=CELEX:52021PC0206&from=EN> ;
    skos:definition "Regulation (EU) 2016/426 of the European Parliament and of the Council of 9 March 2016 on appliances burning gaseous fuels and repealing Directive 2009/142/EC (OJ L 81, 31.3.2016, p. 99);"@en ;
    skos:prefLabel "burning gaseous fuels harmonised legislation"@en .

tair:CablewayInstallationHarmonisedLegislation a tair:Concept ;
    dct:source <https://eur-lex.europa.eu/legal-content/EN/TXT/HTML/?uri=CELEX:52021PC0206&from=EN> ;
    skos:definition "Regulation (EU) 2016/424 of the European Parliament and of the Council of 9 March 2016 on cableway installations and repealing Directive 2000/9/EC (OJ L 81, 31.3.2016, p. 1);"@en ;
    skos:prefLabel "cableway installation harmonised legislation"@en .

tair:CeMarking a tair:Concept ;
    dct:source <https://eur-lex.europa.eu/legal-content/EN/TXT/HTML/?uri=CELEX:52021PC0206&from=EN> ;
    skos:definition "a marking by which a provider indicates that an AI system is in conformity with the requirements set out in Title III, Chapter 2 of this Regulation and other applicable Union legislation harmonising the conditions for the marketing of products ('Union harmonisation legislation') providing for its affixing;"@en ;
    skos:prefLabel "CE marking"@en ;
    skos:related tair:AiSystem .

tair:CivilAviationHarmonisedLegislation a tair:Concept ;
    dct:source <https://eur-lex.europa.eu/legal-content/EN/TXT/HTML/?uri=CELEX:52021PC0206&from=EN> ;
    skos:definition "Regulation (EC) No 300/2008 of the European Parliament and of the Council of 11 March 2008 on common rules in the field of civil aviation security and repealing Regulation (EC) No 2320/2002 (OJ L 97, 9.4.2008, p. 72)."@en ;
    skos:prefLabel "civil aviation harmonised legislation"@en .

tair:CivilAviationSafetyHarmonisedLegislation a tair:Concept ;
    dct:source <https://eur-lex.europa.eu/legal-content/EN/TXT/HTML/?uri=CELEX:52021PC0206&from=EN> ;
    skos:definition "Regulation (EU) 2018/1139 of the European Parliament and of the Council of 4 July 2018 on common rules in the field of civil aviation and establishing a European Union Aviation Safety Agency, and amending Regulations (EC) No 2111/2005, (EC) No 1008/2008, (EU) No 996/2010, (EU) No 376/2014 and Directives 2014/30/EU and 2014/53/EU of the European Parliament and of the Council, and repealing Regulations (EC) No 552/2004 and (EC) No 216/2008 of the European Parliament and of the Council and Council Regulation (EEC) No 3922/91 (OJ L 212, 22.8.2018, p. 1), in so far as the design, production and placing on the market of aircrafts referred to in points (a) and (b) of Article 2(1) thereof, where it concerns unmanned aircraft and their engines, propellers, parts and equipment to control them remotely, are concerned."@en ;
    skos:prefLabel "civil aviation safety harmonised legislation"@en .

tair:CommonSpecification a tair:Concept ;
    dct:source <https://eur-lex.europa.eu/legal-content/EN/TXT/HTML/?uri=CELEX:52021PC0206&from=EN> ;
    skos:definition "a document, other than a standard, containing technical solutions providing a means to, comply with certain requirements and obligations established under this Regulation"@en ;
    skos:prefLabel "common specification"@en .

tair:CrimePredictionAiSystem a tair:Concept ;
    dct:source <https://eur-lex.europa.eu/legal-content/EN/TXT/HTML/?uri=CELEX:52021PC0206&from=EN> ;
    skos:broader tair:AiSystem,
        tair:LawEnforcementHighRiskAreas ;
    skos:definition "AI systems intended to be used by law enforcement authorities for predicting the occurrence or reoccurrence of an actual or potential criminal offence based on profiling of natural persons as referred to in Article 3(4) of Directive (EU) 2016/680 or assessing personality traits and characteristics or past criminal behaviour of natural persons or groups;"@en ;
    skos:prefLabel "crime prediction"@en .

tair:CriminalDataAnalysisAiSystem a tair:Concept ;
    dct:source <https://eur-lex.europa.eu/legal-content/EN/TXT/HTML/?uri=CELEX:52021PC0206&from=EN> ;
    skos:broader tair:AiSystem,
        tair:LawEnforcementHighRiskAreas ;
    skos:definition "AI systems intended to be used for crime analytics regarding natural persons, allowing law enforcement authorities to search complex related and unrelated large data sets available in different data sources or in different data formats in order to identify unknown patterns or discover hidden relationships in the data."@en ;
    skos:prefLabel "criminal data analysis"@en .

tair:CriticalInfrastructureHighRiskArea a tair:Concept ;
    dct:source <https://eur-lex.europa.eu/legal-content/EN/TXT/HTML/?uri=CELEX:52021PC0206&from=EN> ;
    skos:definition "Management and operation of critical infrastructure"@en ;
    skos:prefLabel "management and operation of critical infrastructure"@en ;
    skos:related tair:AiSystem .

tair:DecisionOnCreditAssessmentAiSystem a tair:Concept ;
    dct:source <https://eur-lex.europa.eu/legal-content/EN/TXT/HTML/?uri=CELEX:52021PC0206&from=EN> ;
    skos:broader tair:AccessToEssentialServicesAndBenefitsHighRiskArea,
        tair:AiSystem ;
    skos:definition "AI systems intended to be used to evaluate the creditworthiness of natural persons or establish their credit score, with the exception of AI systems put into service by small scale providers for their own use;"@en ;
    skos:prefLabel "credit assessment"@en .

tair:DecisionOnEmergencyServicesAiSystem a tair:Concept ;
    dct:source <https://eur-lex.europa.eu/legal-content/EN/TXT/HTML/?uri=CELEX:52021PC0206&from=EN> ;
    skos:broader tair:AccessToEssentialServicesAndBenefitsHighRiskArea,
        tair:AiSystem ;
    skos:definition "AI systems intended to be used to dispatch, or to establish priority in the dispatching of emergency first response services, including by firefighters and medical aid."@en .

tair:DecisionOnPublicBenefitsAndServicesAiSystem a tair:Concept ;
    dct:source <https://eur-lex.europa.eu/legal-content/EN/TXT/HTML/?uri=CELEX:52021PC0206&from=EN> ;
    skos:broader tair:AccessToEssentialServicesAndBenefitsHighRiskArea,
        tair:AiSystem ;
    skos:definition "AI systems intended to be used by public authorities or on behalf of public authorities to evaluate the eligibility of natural persons for public assistance benefits and services, as well as to grant, reduce, revoke, or reclaim such benefits and services;"@en ;
    skos:prefLabel "decision of public benefits ad services"@en .

tair:DecisionsInmploymentAiSystem a tair:Concept ;
    dct:source <https://eur-lex.europa.eu/legal-content/EN/TXT/HTML/?uri=CELEX:52021PC0206&from=EN> ;
    skos:broader tair:employmentRelatedHighRiskAreas ;
    skos:definition "AI intended to be used for making decisions on promotion and termination of work-related contractual relationships, for task allocation and for monitoring and evaluating performance and behavior of persons in such relationships."@en ;
    skos:prefLabel "decisions in employment"@en .

tair:DeepFakeDetectionForLawEnforcementAiSystem a tair:Concept ;
    dct:source <https://eur-lex.europa.eu/legal-content/EN/TXT/HTML/?uri=CELEX:52021PC0206&from=EN> ;
    skos:broader tair:AiSystem,
        tair:LawEnforcementHighRiskAreas ;
    skos:definition "AI systems intended to be used by law enforcement authorities to detect deep fakes as referred to in article 52(3);"@en ;
    skos:prefLabel "deep fake detection for law enforcement"@en .

tair:Distributor a tair:Concept ;
    dct:source <https://eur-lex.europa.eu/legal-content/EN/TXT/HTML/?uri=CELEX:52021PC0206&from=EN> ;
    skos:broader tair:Operator ;
    skos:definition "any natural or legal person in the supply chain, other than the provider or the importer, that makes an AI system available on the Union market without affecting its properties"@en ;
    skos:prefLabel "distributor"@en ;
    skos:related tair:AiSystem .

tair:EducationAndTrainingHighRiskArea a tair:Concept ;
    dct:source <https://eur-lex.europa.eu/legal-content/EN/TXT/HTML/?uri=CELEX:52021PC0206&from=EN> ;
    skos:definition "Education and vocational training"@en ;
    skos:prefLabel "education and vocational training"@en ;
    skos:related tair:AiSystem .

tair:EmotionDetectionForLawEnforcementAiSystem a tair:Concept ;
    dct:source <https://eur-lex.europa.eu/legal-content/EN/TXT/HTML/?uri=CELEX:52021PC0206&from=EN> ;
    skos:broader tair:AiSystem,
        tair:LawEnforcementHighRiskAreas ;
    skos:definition "AI systems intended to be used by law enforcement authorities as polygraphs and similar tools or to detect the emotional state of a natural person;"@en ;
    skos:prefLabel "emotion detection of law enforcement"@en .

tair:EmotionRecognitionSystem a tair:Concept ;
    dct:source <https://eur-lex.europa.eu/legal-content/EN/TXT/HTML/?uri=CELEX:52021PC0206&from=EN> ;
    skos:broader tair:AiSystem ;
    skos:definition "an AI system for the purpose of identifying or inferring emotions or intentions of natural persons on the basis of their biometric data"@en ;
    skos:prefLabel "emotion recognition system"@en ;
    skos:related tair:BiometricData .

tair:EmploymentRelatedHighRiskArea a tair:Concept ;
    dct:source <https://eur-lex.europa.eu/legal-content/EN/TXT/HTML/?uri=CELEX:52021PC0206&from=EN> ;
    skos:definition "Employment, workers management and access to self-employment"@en ;
    skos:prefLabel "employment, workers management and access to self-employment"@en ;
    skos:related tair:AiSystem .

tair:EvidenceReliabilityAssessmentAiSystem a tair:Concept ;
    dct:source <https://eur-lex.europa.eu/legal-content/EN/TXT/HTML/?uri=CELEX:52021PC0206&from=EN> ;
    skos:broader tair:AiSystem,
        tair:LawEnforcementHighRiskAreas ;
    skos:definition "AI systems intended to be used by law enforcement authorities for evaluation of the reliability of evidence in the course of investigation or prosecution of criminal offences;"@en ;
    skos:prefLabel "evidence reliability assessment"@en .

tair:ExplosiveGassesHarmonisedLegislation a tair:Concept ;
    dct:source <https://eur-lex.europa.eu/legal-content/EN/TXT/HTML/?uri=CELEX:52021PC0206&from=EN> ;
    skos:definition "Directive 2014/34/EU of the European Parliament and of the Council of 26 February 2014 on the harmonisation of the laws of the Member States relating to equipment and protective systems intended for use in potentially explosive atmospheres (OJ L 96, 29.3.2014, p. 309);"@en ;
    skos:prefLabel "Explosive gasses"@en .

tair:HarmonisedStandard a tair:Concept ;
    dct:source <https://eur-lex.europa.eu/legal-content/EN/TXT/HTML/?uri=CELEX:52021PC0206&from=EN> ;
    skos:definition "a European standard as defined in Article 2(1)(c) of Regulation (EU) No 1025/2012"@en ;
    skos:prefLabel "harmonised standard"@en ;
    skos:scopeNote "Article 2(1)(c) of Regulation (EU) No 1025/2012 states: ‘harmonised standard’ means a European standard adopted on the basis of a request made by the Commission for the application of Union harmonisation legislation"@en .

tair:ImmigrationApplicationProcessingAiSystem a tair:Concept ;
    dct:source <https://eur-lex.europa.eu/legal-content/EN/TXT/HTML/?uri=CELEX:52021PC0206&from=EN> ;
    skos:broader tair:AiSystem,
        tair:MigrationAsylumAndBorderControlHighRiskAreas ;
    skos:definition "AI systems intended to assist competent public authorities for the examination of applications for asylum, visa and residence permits and associated complaints with regard to the eligibility of the natural persons applying for a status."@en ;
    skos:prefLabel "immigration status application processing"@en .

tair:ImmigrationDocumentCheckAiSystem a tair:Concept ;
    dct:source <https://eur-lex.europa.eu/legal-content/EN/TXT/HTML/?uri=CELEX:52021PC0206&from=EN> ;
    skos:broader tair:AiSystem,
        tair:MigrationAsylumAndBorderControlHighRiskAreas ;
    skos:definition "AI systems intended to be used by competent public authorities for the verification of the authenticity of travel documents and supporting documentation of natural persons and detect non-authentic documents by checking their security features;"@en ;
    skos:prefLabel "immigration documentation checking"@en .

tair:Importer a tair:Concept ;
    dct:source <https://eur-lex.europa.eu/legal-content/EN/TXT/HTML/?uri=CELEX:52021PC0206&from=EN> ;
    skos:broader tair:Operator ;
    skos:definition "any natural or legal person established in the Union that places on the market or puts into service an AI system that bears the name or trademark of a natural or legal person established outside the Union"@en ;
    skos:prefLabel "importer"@en ;
    skos:related tair:AiSystem .

tair:InVitroDiagnosticMedicalDevicesHarmonisedLegislation a tair:Concept ;
    dct:source <https://eur-lex.europa.eu/legal-content/EN/TXT/HTML/?uri=CELEX:52021PC0206&from=EN> ;
    skos:definition "Regulation (EU) 2017/746 of the European Parliament and of the Council of 5 April 2017 on in vitro diagnostic medical devices and repealing Directive 98/79/EC and Commission Decision 2010/227/EU (OJ L 117, 5.5.2017, p. 176)."@en ;
    skos:prefLabel "in vitro diagnostic medical devices harmonised legislation"@en .

tair:InputData a tair:Concept ;
    dct:source <https://eur-lex.europa.eu/legal-content/EN/TXT/HTML/?uri=CELEX:52021PC0206&from=EN> ;
    skos:definition "data provided to or directly acquired by an AI system on the basis of which the system produces an output"@en ;
    skos:prefLabel "input data"@en ;
    skos:related tair:AiSystem .

tair:InstructionsForUse a tair:Concept ;
    dct:source <https://eur-lex.europa.eu/legal-content/EN/TXT/HTML/?uri=CELEX:52021PC0206&from=EN> ;
    skos:definition "the information provided by the provider to inform the user of in particular an AI system's intended purpose and proper use, inclusive of the specific geographical, behavioural or functional setting within which the high-risk AI system is intended to be used"@en ;
    skos:prefLabel "instructions for use"@en ;
    skos:related tair:AiSystem,
        tair:User .

tair:JudicialAuthorityAssistanceAiSystem a tair:Concept ;
    dct:source <https://eur-lex.europa.eu/legal-content/EN/TXT/HTML/?uri=CELEX:52021PC0206&from=EN> ;
    skos:broader tair:AdministrationOfJusticeAndDemocraticHighRiskAreas,
        tair:AiSystem ;
    skos:definition "AI systems intended to assist a judicial authority in researching and interpreting facts and the law and in applying the law"@en ;
    skos:prefLabel "assistance for judicial authority"@en .

tair:LawEnforcementHighRiskArea a tair:Concept ;
    dct:source <https://eur-lex.europa.eu/legal-content/EN/TXT/HTML/?uri=CELEX:52021PC0206&from=EN> ;
    skos:definition "Law enforcement:"@en ;
    skos:prefLabel "law enforcement"@en ;
    skos:related tair:AiSystem .

tair:LieAndEmotionDetectionForImmigrationAiSystem a tair:Concept ;
    dct:source <https://eur-lex.europa.eu/legal-content/EN/TXT/HTML/?uri=CELEX:52021PC0206&from=EN> ;
    skos:broader tair:AiSystem,
        tair:MigrationAsylumAndBorderControlHighRiskAreas ;
    skos:definition "AI systems intended to be used by competent public authorities as polygraphs and similar tools or to detect the emotional state of a natural person;"@en ;
    skos:prefLabel "lie and emotion detection for immigration"@en .

tair:LiftsHarmonisedLegislation a tair:Concept ;
    dct:source <https://eur-lex.europa.eu/legal-content/EN/TXT/HTML/?uri=CELEX:52021PC0206&from=EN> ;
    skos:definition "Directive 2014/33/EU of the European Parliament and of the Council of 26 February 2014 on the harmonisation of the laws of the Member States relating to lifts and safety components for lifts (OJ L 96, 29.3.2014, p. 251);"@en ;
    skos:prefLabel "Lifts"@en .

tair:LogicAndKowledgeBasedApproaches a tair:Concept ;
    dct:source <https://eur-lex.europa.eu/legal-content/EN/TXT/HTML/?uri=CELEX:52021PC0206&from=EN> ;
    skos:broader tair:AiSystem ;
    skos:definition "Logic- and knowledge-based approaches, including knowledge representation, inductive (logic) programming, knowledge bases, inference and deductive engines, (symbolic) reasoning and expert systems"@en ;
    skos:prefLabel "logic- and knowledge-based approaches"@en .

tair:MachineLearningApproaches a tair:Concept ;
    dct:source <https://eur-lex.europa.eu/legal-content/EN/TXT/HTML/?uri=CELEX:52021PC0206&from=EN> ;
    skos:broader tair:AiSystem ;
    skos:definition "Machine learning approaches, including supervised, unsupervised and reinforcement learning, using a wide variety of methods including deep learning"@en ;
    skos:prefLabel "machine learning approaches"@en .

tair:MachineryHarmonisedLegislation a tair:Concept ;
    dct:source <https://eur-lex.europa.eu/legal-content/EN/TXT/HTML/?uri=CELEX:52021PC0206&from=EN> ;
    skos:definition "Directive 2006/42/EC of the European Parliament and of the Council of 17 May 2006 on machinery, and amending Directive 95/16/EC (OJ L 157, 9.6.2006, p. 24) [as repealed by the Machinery Regulation];"@en ;
    skos:prefLabel "Machinery"@en .

tair:MakingAvailableOnTheMarket a tair:Concept ;
    dct:source <https://eur-lex.europa.eu/legal-content/EN/TXT/HTML/?uri=CELEX:52021PC0206&from=EN> ;
    skos:definition "any supply of an AI system for distribution or use on the Union market in the course of a commercial activity, whether in return for payment or free of charge"@en ;
    skos:prefLabel "making available on the market"@en ;
    skos:related tair:AiSystem .

tair:MarineEquipmentHarmonisedLegislation a tair:Concept ;
    dct:source <https://eur-lex.europa.eu/legal-content/EN/TXT/HTML/?uri=CELEX:52021PC0206&from=EN> ;
    skos:definition "Directive 2014/90/EU of the European Parliament and of the Council of 23 July 2014 on marine equipment and repealing Council Directive 96/98/EC (OJ L 257, 28.8.2014, p. 146);"@en ;
    skos:prefLabel "marine equipment harmonised legislation"@en .

tair:MarketSurveillanceAuthority a tair:Concept ;
    dct:source <https://eur-lex.europa.eu/legal-content/EN/TXT/HTML/?uri=CELEX:52021PC0206&from=EN> ;
    skos:definition "the national authority carrying out the activities and taking the measures pursuant to Regulation (EU) 2019/1020"@en ;
    skos:prefLabel "market surveillance authority"@en .

tair:MedicalDevicesHarmonisedLegislation a tair:Concept ;
    dct:source <https://eur-lex.europa.eu/legal-content/EN/TXT/HTML/?uri=CELEX:52021PC0206&from=EN> ;
    skos:definition "Regulation (EU) 2017/745 of the European Parliament and of the Council of 5 April 2017 on medical devices, amending Directive 2001/83/EC, Regulation (EC) No 178/2002 and Regulation (EC) No 1223/2009 and repealing Council Directives 90/385/EEC and 93/42/EEC (OJ L 117, 5.5.2017, p. 1;"@en ;
    skos:prefLabel "medical devices harmonised legislation"@en .

tair:MigrationAsylumAndBorderControlHighRiskArea a tair:Concept ;
    dct:source <https://eur-lex.europa.eu/legal-content/EN/TXT/HTML/?uri=CELEX:52021PC0206&from=EN> ;
    skos:definition "Migration, asylum and border control management:"@en ;
    skos:prefLabel "migration, asylum and border control management"@en ;
    skos:related tair:AiSystem .

tair:MotorVehiclesAndTheirTrailersAndComponentsHarmonisedLegislation a tair:Concept ;
    dct:source <https://eur-lex.europa.eu/legal-content/EN/TXT/HTML/?uri=CELEX:52021PC0206&from=EN> ;
    skos:definition "Regulation (EU) 2018/858 of the European Parliament and of the Council of 30 May 2018 on the approval and market surveillance of motor vehicles and their trailers, and of systems, components and separate technical units intended for such vehicles, amending Regulations (EC) No 715/2007 and (EC) No 595/2009 and repealing Directive 2007/46/EC (OJ L 151, 14.6.2018, p. 1); 3. Regulation (EU) 2019/2144 of the European Parliament and of the Council of 27 November 2019 on type-approval requirements for motor vehicles and their trailers, and systems, components and separate technical units intended for such vehicles, as regards their general safety and the protection of vehicle occupants and vulnerable road users, amending Regulation (EU) 2018/858 of the European Parliament and of the Council and repealing Regulations (EC) No 78/2009, (EC) No 79/2009 and (EC) No 661/2009 of the European Parliament and of the Council and Commission Regulations (EC) No 631/2009, (EU) No 406/2010, (EU) No 672/2010, (EU) No 1003/2010, (EU) No 1005/2010, (EU) No 1008/2010, (EU) No 1009/2010, (EU) No 19/2011, (EU) No 109/2011, (EU) No 458/2011, (EU) No 65/2012, (EU) No 130/2012, (EU) No 347/2012, (EU) No 351/2012, (EU) No 1230/2012 and (EU) 2015/166 (OJ L 325, 16.12.2019, p. 1);"@en ;
    skos:prefLabel "motor vehicles and their trailers and components harmonised legislation"@en .

tair:NationalCompetentAuthority a tair:Concept ;
    dct:source <https://eur-lex.europa.eu/legal-content/EN/TXT/HTML/?uri=CELEX:52021PC0206&from=EN> ;
    skos:definition "the national supervisory authority, the notifying authority and the market surveillance authority"@en ;
    skos:prefLabel "national competent authority"@en .

tair:NationalSupervisoryAuthority a tair:Concept ;
    dct:source <https://eur-lex.europa.eu/legal-content/EN/TXT/HTML/?uri=CELEX:52021PC0206&from=EN> ;
    skos:definition "means the authority to which a Member State assigns the responsibility for the implementation and application of this Regulation, for coordinating the activities entrusted to that Member State, for acting as the single contact point for the Commission, and for representing the Member State at the European Artificial Intelligence Board"@en ;
    skos:prefLabel "national supervisory authority"@en .

tair:NotifiedBody a tair:Concept ;
    dct:source <https://eur-lex.europa.eu/legal-content/EN/TXT/HTML/?uri=CELEX:52021PC0206&from=EN> ;
    skos:broader tair:ConformityAssessmentBody ;
    skos:definition "a conformity assessment body designated in accordance with this Regulation and other relevant Union harmonisation legislation"@en ;
    skos:prefLabel "notified body"@en .

tair:NotifyingAuthority a tair:Concept ;
    dct:source <https://eur-lex.europa.eu/legal-content/EN/TXT/HTML/?uri=CELEX:52021PC0206&from=EN> ;
    skos:definition "the national authority responsible for setting up and carrying out the necessary procedures for the assessment, designation and notification of conformity assessment bodies and for their monitoring"@en ;
    skos:prefLabel "notifying authority"@en ;
    skos:related tair:ConformityAssessmentBody .

tair:OffencesRiskAssessmentAiSystem a tair:Concept ;
    dct:source <https://eur-lex.europa.eu/legal-content/EN/TXT/HTML/?uri=CELEX:52021PC0206&from=EN> ;
    skos:broader tair:AiSystem,
        tair:LawEnforcementHighRiskAreas ;
    skos:definition "AI systems intended to be used by law enforcement authorities for making individual risk assessments of natural persons in order to assess the risk of a natural person for offending or reoffending or the risk for potential victims of criminal offences;"@en ;
    skos:prefLabel "risk assessment for offences"@en .

tair:Performance a tair:Concept ;
    dct:source <https://eur-lex.europa.eu/legal-content/EN/TXT/HTML/?uri=CELEX:52021PC0206&from=EN> ;
    skos:definition "the ability of an AI system to achieve its intended purpose"@en ;
    skos:prefLabel "performance"@en ;
    skos:related tair:AiSystem .

tair:PersonalProtectiveEquipmentHarmonisedLegislation a tair:Concept ;
    dct:source <https://eur-lex.europa.eu/legal-content/EN/TXT/HTML/?uri=CELEX:52021PC0206&from=EN> ;
    skos:definition "Regulation (EU) 2016/425 of the European Parliament and of the Council of 9 March 2016 on personal protective equipment and repealing Council Directive 89/686/EEC (OJ L 81, 31.3.2016, p. 51);"@en ;
    skos:prefLabel "personal protective equipment harmonised legislation"@en .

tair:PlacingOnTheMarket a tair:Concept ;
    dct:source <https://eur-lex.europa.eu/legal-content/EN/TXT/HTML/?uri=CELEX:52021PC0206&from=EN> ;
    skos:definition "the first making available of an AI system on the Union market"@en ;
    skos:prefLabel "placing on the market"@en ;
    skos:related tair:AiSystem .

tair:PostMarketMonitoring a tair:Concept ;
    dct:source <https://eur-lex.europa.eu/legal-content/EN/TXT/HTML/?uri=CELEX:52021PC0206&from=EN> ;
    skos:definition "all activities carried out by providers of AI systems to proactively collect and review experience gained from the use of AI systems they place on the market or put into service for the purpose of identifying any need to immediately apply any necessary corrective or preventive actions"@en ;
    skos:prefLabel "post-market monitoring"@en ;
    skos:related tair:AiSystem .

tair:PostRemoteBiometricIdentificationSystem a tair:Concept ;
    dct:source <https://eur-lex.europa.eu/legal-content/EN/TXT/HTML/?uri=CELEX:52021PC0206&from=EN> ;
    skos:broader tair:RemoteBiometricIdentificationSystem ;
    skos:definition "a remote biometric identification system other than a 'real-time' remote biometric identification system"@en ;
    skos:prefLabel "post remote biometric identification system"@en .

tair:PressureEquipmentHarmonisedLegislation a tair:Concept ;
    dct:source <https://eur-lex.europa.eu/legal-content/EN/TXT/HTML/?uri=CELEX:52021PC0206&from=EN> ;
    skos:definition "Directive 2014/68/EU of the European Parliament and of the Council of 15 May 2014 on the harmonisation of the laws of the Member States relating to the making available on the market of pressure equipment (OJ L 189, 27.6.2014, p. 164);"@en ;
    skos:prefLabel "pressure equipment harmonised legislation"@en .

tair:ProfilingForLawEnforcementAiSystem a tair:Concept ;
    dct:source <https://eur-lex.europa.eu/legal-content/EN/TXT/HTML/?uri=CELEX:52021PC0206&from=EN> ;
    skos:broader tair:AiSystem,
        tair:LawEnforcementHighRiskAreas ;
    skos:definition "AI systems intended to be used by law enforcement authorities for profiling of natural persons as referred to in Article 3(4) of Directive (EU) 2016/680 in the course of detection, investigation or prosecution of criminal offences;"@en ;
    skos:prefLabel "profiling for law enforcement"@en .

tair:PubliclyAccessibleSpace a tair:Concept ;
    dct:source <https://eur-lex.europa.eu/legal-content/EN/TXT/HTML/?uri=CELEX:52021PC0206&from=EN> ;
    skos:definition "any physical place accessible to the public, regardless of whether certain conditions for access may apply"@en ;
    skos:prefLabel "publicly accessible space"@en .

tair:PuttingIntoService a tair:Concept ;
    dct:source <https://eur-lex.europa.eu/legal-content/EN/TXT/HTML/?uri=CELEX:52021PC0206&from=EN> ;
    skos:definition "the supply of an AI system for first use directly to the user or for own use on the Union market for its intended purpose"@en ;
    skos:prefLabel "putting into service"@en ;
    skos:related tair:AiSystem .

tair:RadioEquipmentHarmonisedLegislation a tair:Concept ;
    dct:source <https://eur-lex.europa.eu/legal-content/EN/TXT/HTML/?uri=CELEX:52021PC0206&from=EN> ;
    skos:definition "Directive 2014/53/EU of the European Parliament and of the Council of 16 April 2014 on the harmonisation of the laws of the Member States relating to the making available on the market of radio equipment and repealing Directive 1999/5/EC (OJ L 153, 22.5.2014, p. 62);"@en ;
    skos:prefLabel "radio equipment harmonised legislation"@en .

tair:RailSystemsHarmonisedLegislation a tair:Concept ;
    dct:source <https://eur-lex.europa.eu/legal-content/EN/TXT/HTML/?uri=CELEX:52021PC0206&from=EN> ;
    skos:definition "Directive (EU) 2016/797 of the European Parliament and of the Council of 11 May 2016 on the interoperability of the rail system within the European Union (OJ L 138, 26.5.2016, p. 44)."@en ;
    skos:prefLabel "rail systems harmonised legislation"@en .

tair:RealTimeRemoteBiometricIdentificationSystem a tair:Concept ;
    dct:source <https://eur-lex.europa.eu/legal-content/EN/TXT/HTML/?uri=CELEX:52021PC0206&from=EN> ;
    skos:broader tair:RemoteBiometricIdentificationSystem ;
    skos:definition "a remote biometric identification system whereby the capturing of biometric data, the comparison and the identification all occur without a significant delay. This comprises not only instant identification, but also limited short delays in order to avoid circumvention"@en ;
    skos:prefLabel "real-time' remote biometric identification system"@en ;
    skos:related tair:BiometricData .

tair:ReasonablyForseeableMisuse a tair:Concept ;
    dct:source <https://eur-lex.europa.eu/legal-content/EN/TXT/HTML/?uri=CELEX:52021PC0206&from=EN> ;
    skos:definition "the use of an AI system in a way that is not in accordance with its intended purpose, but which may result from reasonably foreseeable human behaviour or interaction with other systems"@en ;
    skos:prefLabel "resonably forseeable misuse"@en ;
    skos:related tair:AiSystem,
        tair:IntendedPurpose .

tair:Recall a tair:Concept ;
    dct:source <https://eur-lex.europa.eu/legal-content/EN/TXT/HTML/?uri=CELEX:52021PC0206&from=EN> ;
    skos:definition "any measure aimed at achieving the return to the provider of an AI system made available to users"@en ;
    skos:prefLabel "recall of an AI system"@en ;
    skos:related tair:AiSystem,
        tair:Provider,
        tair:User .

tair:RecreationalPersonalWatercraftHarmonisedLegislation a tair:Concept ;
    dct:source <https://eur-lex.europa.eu/legal-content/EN/TXT/HTML/?uri=CELEX:52021PC0206&from=EN> ;
    skos:definition "Directive 2013/53/EU of the European Parliament and of the Council of 20 November 2013 on recreational craft and personal watercraft and repealing Directive 94/25/EC (OJ L 354, 28.12.2013, p. 90);"@en ;
    skos:prefLabel "Recreational/Personal watercraft"@en .

tair:RecruitmentForEmploymentAiSystem a tair:Concept ;
    dct:source <https://eur-lex.europa.eu/legal-content/EN/TXT/HTML/?uri=CELEX:52021PC0206&from=EN> ;
    skos:broader tair:AiSystem,
        tair:employmentRelatedHighRiskAreas ;
    skos:definition "AI systems intended to be used for recruitment or selection of natural persons, notably for advertising vacancies, screening or filtering applications, evaluating candidates in the course of interviews or tests"@en ;
    skos:prefLabel "recruitment for employment"@en .

tair:RemoteBiometricIdAiSystem a tair:Concept ;
    dct:source <https://eur-lex.europa.eu/legal-content/EN/TXT/HTML/?uri=CELEX:52021PC0206&from=EN> ;
    skos:broader tair:AiSystem,
        tair:BiometricIdHighRiskAreas ;
    skos:definition "AI systems intended to be used for the ‘real-time’ and ‘post’ remote biometric identification of natural persons"@en ;
    skos:prefLabel "remote biometric identification of natural persons"@en .

tair:SafetyComponent a tair:Concept ;
    dct:source <https://eur-lex.europa.eu/legal-content/EN/TXT/HTML/?uri=CELEX:52021PC0206&from=EN> ;
    skos:definition "a component of a product or of a system which fulfils a safety function for that product or system or the failure or malfunctioning of which endangers the health and safety of persons or property"@en ;
    skos:prefLabel "safety component of a product or service"@en .

tair:SafetyOfCriticalInfrastructureAiSystem a tair:Concept ;
    dct:source <https://eur-lex.europa.eu/legal-content/EN/TXT/HTML/?uri=CELEX:52021PC0206&from=EN> ;
    skos:broader tair:AiSystem,
        tair:CriticalInfrastructureHighRiskAreas ;
    skos:definition "AI systems intended to be used as safety components in the management and operation of road traffic and the supply of water, gas, heating and electricity"@en ;
    skos:prefLabel "safety components of critical infrastructure"@en .

tair:SecurityImmigrationAndHealthRiskAiSystem a tair:Concept ;
    dct:source <https://eur-lex.europa.eu/legal-content/EN/TXT/HTML/?uri=CELEX:52021PC0206&from=EN> ;
    skos:broader tair:AiSystem,
        tair:MigrationAsylumAndBorderControlHighRiskAreas ;
    skos:definition "AI systems intended to be used by competent public authorities to assess a risk, including a security risk, a risk of irregular immigration, or a health risk, posed by a natural person who intends to enter or has entered into the territory of a Member State;"@en ;
    skos:prefLabel "secuirty, immigration or health risk assessment"@en .

tair:SeriousIncidentInfrastructure a tair:Concept ;
    dct:source <https://eur-lex.europa.eu/legal-content/EN/TXT/HTML/?uri=CELEX:52021PC0206&from=EN> ;
    skos:definition "a serious and irreversible disruption of the management and operation of critical infrastructure"@en ;
    skos:prefLabel "serious incident to critical infrastructure"@en .

tair:SeriousIncidentPersonPropertyEnvironment a tair:Concept ;
    dct:source <https://eur-lex.europa.eu/legal-content/EN/TXT/HTML/?uri=CELEX:52021PC0206&from=EN> ;
    skos:definition "the death of a person or serious damage to a person's health, to property or the environment"@en ;
    skos:prefLabel "serious incident to person, propert or environment"@en .

tair:SmallScaleProvider a tair:Concept ;
    dct:source <https://eur-lex.europa.eu/legal-content/EN/TXT/HTML/?uri=CELEX:52021PC0206&from=EN> ;
    skos:broader tair:Provider ;
    skos:definition "a provider that is a micro or small enterprise within the meaning of Commission Recommendation 2003/361/EC 61"@en ;
    skos:prefLabel "small scale provider"@en .

tair:StatisticalApproaches a tair:Concept ;
    dct:source <https://eur-lex.europa.eu/legal-content/EN/TXT/HTML/?uri=CELEX:52021PC0206&from=EN> ;
    skos:broader tair:AiSystem ;
    skos:definition "Statistical approaches, Bayesian estimation, search and optimization methods"@en ;
    skos:prefLabel "statistical appraoches"@en .

tair:SubstantialChange a tair:Concept ;
    dct:source <https://eur-lex.europa.eu/legal-content/EN/TXT/HTML/?uri=CELEX:52021PC0206&from=EN> ;
    skos:definition "a change to the AI system following its placing on the market or putting into service which affects the compliance of the AI system with the requirements set out in Title III, Chapter 2 of this Regulation or results in a modification to the intended purpose for which the AI system has been assessed"@en ;
    skos:prefLabel "substantial change"@en ;
    skos:related tair:AiSystem .

tair:TestingData a tair:Concept ;
    dct:source <https://eur-lex.europa.eu/legal-content/EN/TXT/HTML/?uri=CELEX:52021PC0206&from=EN> ;
    skos:definition "data used for providing an independent evaluation of the trained and validated AI system in order to confirm the expected performance of that system before its placing on the market or putting into service"@en ;
    skos:prefLabel "testing data"@en ;
    skos:related tair:AiSystem .

tair:ToysHarmonisedLegislation a tair:Concept ;
    dct:source <https://eur-lex.europa.eu/legal-content/EN/TXT/HTML/?uri=CELEX:52021PC0206&from=EN> ;
    skos:definition "Directive 2009/48/EC of the European Parliament and of the Council of 18 June 2009 on the safety of toys (OJ L 170, 30.6.2009, p. 1);"@en ;
    skos:prefLabel "Toys"@en .

tair:TrainingData a tair:Concept ;
    dct:source <https://eur-lex.europa.eu/legal-content/EN/TXT/HTML/?uri=CELEX:52021PC0206&from=EN> ;
    skos:definition "data used for training an AI system through fitting its learnable parameters, including the weights of a neural network"@en ;
    skos:prefLabel "training data"@en ;
    skos:related tair:AiSystem .

tair:TwoOrThreeWheelVehiclesAndQuadricyclesHarmonisedLegislation a tair:Concept ;
    dct:source <https://eur-lex.europa.eu/legal-content/EN/TXT/HTML/?uri=CELEX:52021PC0206&from=EN> ;
    skos:definition "Regulation (EU) No 168/2013 of the European Parliament and of the Council of 15 January 2013 on the approval and market surveillance of two- or three-wheel vehicles and quadricycles (OJ L 60, 2.3.2013, p. 52);"@en ;
    skos:prefLabel "two- or three-wheel vehicles and quadricycles harmonised legislation"@en .

tair:ValidationData a tair:Concept ;
    dct:source <https://eur-lex.europa.eu/legal-content/EN/TXT/HTML/?uri=CELEX:52021PC0206&from=EN> ;
    skos:definition "data used for providing an evaluation of the trained AI system and for tuning its non-learnable parameters and its learning process, among other things, in order to prevent overfitting; whereas the validation dataset can be a separate dataset or part of the training dataset, either as a fixed or variable split"@en ;
    skos:prefLabel "validation data"@en ;
    skos:related tair:AiSystem .

tair:Withdrawal a tair:Concept ;
    dct:source <https://eur-lex.europa.eu/legal-content/EN/TXT/HTML/?uri=CELEX:52021PC0206&from=EN> ;
    skos:definition "means any measure aimed at preventing the distribution, display and offer of an AI system"@en ;
    skos:prefLabel "withdrawal"@en ;
    skos:related tair:AiSystem .

tair:ConceptCollection a skos:Collection ;
    prov:wasDerivedFrom <https://eur-lex.europa.eu/legal-content/EN/TXT/HTML/?uri=CELEX:52021PC0206&from=EN> .

tair:ConformityAssessment a tair:Concept ;
    dct:source <https://eur-lex.europa.eu/legal-content/EN/TXT/HTML/?uri=CELEX:52021PC0206&from=EN> ;
    skos:definition "the process of verifying whether the requirements set out in Title III, Chapter 2 of this Regulation relating to an AI system have been fulfilled"@en ;
    skos:prefLabel "conformity assessment"@en ;
    skos:related tair:AiSystem .

tair:IntendedPurpose a tair:Concept ;
    dct:source <https://eur-lex.europa.eu/legal-content/EN/TXT/HTML/?uri=CELEX:52021PC0206&from=EN> ;
    skos:definition "the use for which an AI system is intended by the provider, including the specific context and conditions of use, as specified in the information supplied by the provider in the instructions for use, promotional or sales materials and statements, as well as in the technical documentation"@en ;
    skos:prefLabel "intended purpose"@en ;
    skos:related tair:AiSystem .

tair:LawEnforcementAuthorityOther a tair:Concept ;
    dct:source <https://eur-lex.europa.eu/legal-content/EN/TXT/HTML/?uri=CELEX:52021PC0206&from=EN> ;
    skos:broader tair:LawEnforcement ;
    skos:definition "any other body or entity entrusted by Member State law to exercise public authority and public powers for the purposes of the prevention, investigation, detection or prosecution of criminal offences or the execution of criminal penalties, including the safeguarding against and the prevention of threats to public security"@en ;
    skos:prefLabel "other law enforcement authority"@en ;
    skos:related tair:LawEnforcementAuthorityPublic .

tair:LawEnforcementAuthorityPublic a tair:Concept ;
    dct:source <https://eur-lex.europa.eu/legal-content/EN/TXT/HTML/?uri=CELEX:52021PC0206&from=EN> ;
    skos:broader tair:LawEnforcement ;
    skos:definition "any public authority competent for the prevention, investigation, detection or prosecution of criminal offences or the execution of criminal penalties, including the safeguarding against and the prevention of threats to public security"@en ;
    skos:prefLabel "public law enforcement authority "@en ;
    skos:related tair:LawEnforcementAuthorityOther .

tair:ConformityAssessmentBody a tair:Concept ;
    dct:source <https://eur-lex.europa.eu/legal-content/EN/TXT/HTML/?uri=CELEX:52021PC0206&from=EN> ;
    skos:definition "a body that performs third-party conformity assessment activities, including testing, certification and inspection"@en ;
    skos:prefLabel "conformity assessment body"@en ;
    skos:related tair:ConformityAssessment .

tair:LawEnforcement a tair:Concept ;
    dct:source <https://eur-lex.europa.eu/legal-content/EN/TXT/HTML/?uri=CELEX:52021PC0206&from=EN> ;
    skos:definition "activities carried out by law enforcement authorities for the prevention, investigation, detection or prosecution of criminal offences or the execution of criminal penalties, including the safeguarding against and the prevention of threats to public security"@en ;
    skos:prefLabel "law enforcement"@en .

tair:RemoteBiometricIdentificationSystem a tair:Concept ;
    dct:source <https://eur-lex.europa.eu/legal-content/EN/TXT/HTML/?uri=CELEX:52021PC0206&from=EN> ;
    skos:broader tair:AiSystem ;
    skos:definition "an AI system for the purpose of identifying natural persons at a distance through the comparison of a person's biometric data with the biometric data contained in a reference database, and without prior knowledge of the user of the AI system whether the person will be present and can be identified"@en ;
    skos:prefLabel "remote biometric identification system"@en ;
    skos:related tair:BiometricData .

tair:User a tair:Concept ;
    dct:source <https://eur-lex.europa.eu/legal-content/EN/TXT/HTML/?uri=CELEX:52021PC0206&from=EN> ;
    skos:broader tair:Operator ;
    skos:definition "any natural or legal person, public authority, agency or other body using an AI system under its authority, except where the AI system is used in the course of a personal non-professional activity"@en ;
    skos:prefLabel "user"@en ;
    skos:related tair:AiSystem .

tair:AccessToEssentialServicesAndBenefitsHighRiskArea a tair:Concept ;
    dct:source <https://eur-lex.europa.eu/legal-content/EN/TXT/HTML/?uri=CELEX:52021PC0206&from=EN> ;
    skos:definition "Access to and enjoyment of essential private services and public services and benefits"@en ;
    skos:prefLabel "access to and enjoyment of essential private services and public services and benefits"@en ;
    skos:related tair:AiSystem .

tair:Provider a tair:Concept ;
    dct:source <https://eur-lex.europa.eu/legal-content/EN/TXT/HTML/?uri=CELEX:52021PC0206&from=EN> ;
    skos:broader tair:Operator ;
    skos:definition "natural or legal person, public authority, agency or other body that develops an AI system or that has an AI system developed with a view to placing it on the market or putting it into service under its own name or trademark, whether for payment or free of charge"@en ;
    skos:prefLabel "provider"@en ;
    skos:related tair:AiSystem .

tair:BiometricData a tair:Concept ;
    dct:source <https://eur-lex.europa.eu/legal-content/EN/TXT/HTML/?uri=CELEX:52021PC0206&from=EN> ;
    skos:definition "data resulting from specific technical processing relating to the physical, physiological or behavioural characteristics of a natural person, which allow or confirm the unique identification of that natural person, such as facial images or dactyloscopic data"@en ;
    skos:prefLabel "biometric data"@en .

tair:Operator a tair:Concept ;
    dct:source <https://eur-lex.europa.eu/legal-content/EN/TXT/HTML/?uri=CELEX:52021PC0206&from=EN> ;
    skos:definition "the provider, the user, the authorised representative, the importer and the distributor"@en ;
    skos:prefLabel "operator"@en .

tair:AiSystem a tair:Concept ;
    dct:source <https://eur-lex.europa.eu/legal-content/EN/TXT/HTML/?uri=CELEX:52021PC0206&from=EN> ;
    skos:definition "software that is developed with one or more of the techniques and approaches listed in Annex I and can, for a given set of human-defined objectives, generate outputs such as content, predictions, recommendations, or decisions influencing the environments they interact with"@en ;
    skos:prefLabel "artificial intelligence system"@en .

tair:Concept a skos:Concept ;
    rdfs:subClassOf tair:ConceptCollection .

